TM/Code/MatchTM.v
@@ -1,0 +1,396 @@
+Require Import TM.Code.CodeTM.
+
+Require Import TM.Basic.Mono TM.Basic.Nop TM.Basic.Multi.
+Require Import TM.Combinators.Combinators.
+Require Import TM.LiftMN.
+
+Require Import TM.Compound.TMTac.
+Require Import TM.Compound.CopySymbols TM.Compound.MoveToSymbol.
+
+
+
+(* Basic pattern matching *)
+Section MatchSum.
+  Variable X Y : Type.
+  Variable (sigX sigY : finType).
+  Hypothesis (codX : codeable sigX X) (codY : codeable sigY Y).
+
+  Definition MatchSum_R : Rel (tapes (sigX+sigY+bool)^+ 1) (bool * tapes (sigX+sigY+bool)^+ 1) :=
+    Mk_R_p (if? (fun (tin tout : tape (sigX+sigY+bool)^+) =>
+                   forall x : X, tape_encodes (Encode_Sum codX codY) tin (inl x) ->
+                            tape_encodes (Encode_Map codX (@retract_l_l sigX sigY)) tout x)
+              ! (fun (tin tout : tape (sigX+sigY+bool)^+) =>
+                   forall y : Y, tape_encodes (Encode_Sum codX codY) tin (inr y) ->
+                            tape_encodes (Encode_Map codY (@retract_l_r sigX sigY)) tout y)).
+
+  Definition MatchSum : { M : mTM (sigX+sigY+bool)^+ 1 & states M -> bool } :=
+    MATCH (Read_char _)
+          (fun o => match o with
+                 | Some (inl (inr true))  => Write (inr START) tt;; Move _ R true  (* inl *)
+                 | Some (inl (inr false)) => Write (inr START) tt;; Move _ R false (* inr *)
+                 | _ => mono_Nop _ true (* invalid input *)
+                 end).
+
+  Lemma MatchSum_Sem : MatchSum ⊨c(5) MatchSum_R.
+  Proof.
+    eapply RealiseIn_monotone.
+    {
+      unfold MatchSum. eapply Match_RealiseIn. cbn. eapply read_char_sem.
+      instantiate (2 := fun o : option (sigX+sigY+bool)^+ =>
+                          match o with Some (inl (inr true)) => _ | Some (inl (inr false)) => _ | _ => _ end).
+      cbn. intros [ s | ]; cbn.
+      - destruct s as [ s | start]; cbn.
+        + destruct s as [xy | cons]; cbn.
+          * eapply RealiseIn_monotone'. eapply mono_Nop_Sem. omega.
+          * destruct cons; (eapply Seq_RealiseIn; [eapply Write_Sem | eapply Move_Sem]).
+        + eapply RealiseIn_monotone'. eapply mono_Nop_Sem. omega.
+      - eapply RealiseIn_monotone'. eapply mono_Nop_Sem. omega.
+    }
+    {
+      cbn. omega.
+    }
+    {
+      intros tin (yout&tout) H. destruct H as (H1&(t&(H2&H3)&H4)); hnf in *. subst.
+      destruct_tapes; cbn in *.
+      destruct h; cbn in *; TMSimp; eauto. destruct e; cbn in *; TMSimp.
+      destruct s; cbn in *; TMSimp. destruct b; TMSimp; cbn in *.
+      - destruct h0; cbn in *; eauto.
+        + destruct (map inl _) in H1; cbn in H1; congruence.
+        + destruct (map inl _) in H1; cbn in H1; congruence.
+        + destruct (map inl _) in H1; cbn in H1; congruence.
+        + destruct (encode x) eqn:E1; cbn in *.
+          * inv H1. do 2 eexists. split; cbn; eauto. now rewrite E1.
+          * inv H1. do 2 eexists. split; cbn; eauto. now rewrite E1.
+      - destruct h0; cbn in *; eauto.
+        + destruct (map inl _) in H1; cbn in H1; congruence.
+        + destruct (map inl _) in H1; cbn in H1; congruence.
+        + destruct (map inl _) in H1; cbn in H1; congruence.
+        + destruct (encode y) eqn:E1; cbn in *.
+          * inv H1. do 2 eexists. split; cbn; eauto. now rewrite E1.
+          * inv H1. do 2 eexists. split; cbn; eauto. now rewrite E1.
+    }
+  Qed.
+
+
+  (* Constructors *)
+  Section SumConstr.
+
+    Definition ConstrSum_Rel (is_left:bool) : Rel (tapes (sigX+sigY+bool)^+ 1) (unit * tapes (sigX+sigY+bool)^+ 1) :=
+      Mk_R_p (
+          ignoreParam
+            (fun tin tout =>
+               if is_left
+               then forall x : X, tape_encodes (Encode_Map codX (@retract_l_l sigX sigY)) tin x ->
+                             tape_encodes (Encode_Sum codX codY) tout (inl x)
+               else forall y : Y, tape_encodes (Encode_Map codY (@retract_l_r sigX sigY)) tin y ->
+                             tape_encodes (Encode_Sum codX codY) tout (inr y))).
+
+    Definition ConstrSum (is_left:bool) : { M : mTM (sigX+sigY+bool)^+ 1 & states M -> unit } :=
+      Move _ L tt;; Write (inl (inr is_left)) tt;; Move _ L tt;; Write (inr START) tt;; Move _ R tt.
+
+    Lemma ConstrSum_Sem (is_left:bool) : (ConstrSum is_left) ⊨c(9) (ConstrSum_Rel is_left).
+    Proof.
+      eapply RealiseIn_monotone.
+      {
+        eapply Seq_RealiseIn. eapply Move_Sem. eapply Seq_RealiseIn.
+        eapply Write_Sem. eapply Seq_RealiseIn. eapply Move_Sem.
+        eapply Seq_RealiseIn. eapply Write_Sem. eapply Move_Sem.
+      }
+      {
+        cbn. omega.
+      }
+      {
+        TMSimp ( cbn [Vector.nth] in * ). destruct is_left; cbn in *; subst; TMSimp.
+        {
+          destruct h; cbn in *; TMSimp; cbn in *.
+          - destruct (encode _) in H0; cbn in *; congruence.
+          - destruct (encode x) as [ | eX eXs] eqn:E;
+              cbn in *; inv H0; cbv [tape_encodes_r]; cbn; rewrite E; cbn;
+                (destruct x0; cbn; eauto).
+        }
+        {
+          destruct h; cbn in *; TMSimp; cbn in *.
+          - destruct (encode _) in H0; cbn in *; congruence.
+          - destruct (encode y) as [ | eX eXs] eqn:E;
+              cbn in *; inv H0; cbv [tape_encodes_r]; cbn; rewrite E; cbn;
+                (destruct x; cbn; eauto).
+        }
+      }
+    Qed.
+                
+      
+  End SumConstr.
+
+End MatchSum.
+
+
+(* TODO: Match operator for functions *)
+(*
+
+Section MatchSum_Fun.
+
+  Variable n : nat.
+  Variable k : nat.
+
+  Variable (sigX sigY : finType).
+  Variable Z : Type.
+  Variable tpZ : Fin.t n.
+  Hypothesis codZ : codeable (sigX+sigY+bool)^+ Z.
+  Variable parF : param_genT (sigX+sigY+bool)^+ n (S k).
+  Variable f : param_genF Z parF.
+
+  Let f_param1 := Vector.hd parF.
+  Let f_param1T := projT1 (fst f_param1).
+  Let f_param1Enc := projT2 (fst f_param1).
+  Let f_param1Tape := snd f_param1.
+
+  Variable X : Type.
+  Variable codX
+
+  Variable para 
+
+
+End MatchSum_Fun.
+
+
+    
+
+    
+
+    
+
+    
+
+    
+
+    
+
+    
+
+    
+
+    
+
+    
+
+    
+
+    
+
+    
+
+    
+
+    
+
+    
+
+    
+
+    
+
+    
+
+    
+
+    
+
+    
+
+    
+
+    
+
+    
+
+    
+
+    
+
+    
+
+    
+
+    
+
+    
+
+    
+
+    
+
+    
+
+    
+
+    
+
+    
+
+    
+
+    
+
+    
+
+    
+
+    
+
+    
+
+    
+
+    
+
+    
+
+    
+
+    
+
+    
+
+    
+
+    
+
+    
+
+    
+
+    
+
+    
+
+    
+
+    
+
+    
+
+    
+
+    
+
+    
+
+    
+
+    
+
+    
+
+    
+
+    
+
+    
+
+    
+
+    
+
+    
+
+    
+
+    
+
+    
+
+    
+
+    
+
+    
+
+    
+
+    
+
+    
+
+    
+
+    
+
+    
+
+    
+
+    
+
+    
+
+    
+
+    
+
+    
+
+    
+
+    
+
+    
+
+    
+
+    
+
+    
+
+    
+
+    
+
+    
+
+    
+
+    
+
+    
+
+
+Section MatchTM.
+
+  Variable sig : finType.
+  Variable n : nat.
+  Variable (F1 : finType).
+  Variable (def : F1).
+  Variable (pM : sig -> { M1 : mTM sig^+ n & states M1 -> F1}).
+
+  Variable k : nat.
+  Variable resType : Type.
+  Variable resTape : Fin.t n.
+  Hypothesis codRes : codeable sig resType.
+  Variable params : param_genT sig n (S k).
+  Variable f : param_genF resType params.
+
+  Let param1 := Vector.hd params.
+  Let param1T := projT1 (fst param1).
+  Let param1Enc := projT2 (fst param1).
+  Let param1Tape := snd param1.
+
+  Definition matchTM : { M : mTM sig^+ n & states M -> F1}:=
+    MATCH (Read_char_at (sig^+) param1Tape)
+          (fun o : option (sig^+) =>
+             match o with
+             | Some (inl s) =>
+               (* TODO: write True on param1T, move param1T to R, call pM s *)
+               pM s
+             | _ => Nop n _ def
+             end).
+
+
+  Section MatchOption.
+
+    Variable cont_None : 
+    
+  End MatchOption.
+
+End MatchTM.
+
+*)
